Weidenbach_Book/Watched_Literals_Watch_List_Initialisation.thy
@@ -1,5 +1,5 @@
 theory Watched_Literals_Watch_List_Initialisation
-  imports Watched_Literals_Watch_List Watched_Literals_Initialisation "../lib/Explorer"
+  imports Watched_Literals_Watch_List Watched_Literals_Initialisation
 begin
 
 
